Remove explicit `validOnFrameClass` in Modal and Propositional (#247)

Foundation/Modal/Kripke/AxiomWeakPoint3.lean
@@ -55,18 +55,24 @@ lemma validate_WeakPoint3_of_weakConnected : F ⊧ (Axioms.WeakPoint3 (.atom 0) 
     nRyz
   ⟩;
 
-abbrev WeakConnectedFrameClass : FrameClass := { F | WeakConnected F }
+abbrev FrameClass.weakConnected : FrameClass := { F | WeakConnected F }
 
-instance : WeakConnectedFrameClass.IsNonempty := by
-  use ⟨Unit, λ _ _ => True⟩;
+namespace FrameClass.weakConnected
+
+@[simp]
+protected lemma nonempty : FrameClass.weakConnected.Nonempty := by
+  use whitepoint.toFrame;
   simp [WeakConnected];
 
-instance WeakConnectedFrameClass.DefinedByWeakPoint3 : WeakConnectedFrameClass.DefinedBy {Axioms.WeakPoint3 (.atom 0) (.atom 1)} := ⟨by
+protected instance definability : FrameClass.weakConnected.DefinedBy {Axioms.WeakPoint3 (.atom 0) (.atom 1)} := ⟨by
   intro F;
   constructor;
   . simpa using weakConnected_of_validate_WeakPoint3;
   . simpa using validate_WeakPoint3_of_weakConnected;
 ⟩
+
+end FrameClass.weakConnected
+
 
 end definability
 
@@ -83,7 +89,7 @@ open canonicalModel
 
 namespace Canonical
 
-lemma weakConnected [Entailment.HasAxiomWeakPoint3 𝓢] : WeakConnected (canonicalFrame 𝓢).Rel := by
+protected lemma weakConnected [Entailment.HasAxiomWeakPoint3 𝓢] : WeakConnected (canonicalFrame 𝓢).Rel := by
   rintro x y z ⟨Rxy, Rxz, eyz⟩;
   by_contra hC;
   push_neg at hC;
