Foundation/Modal/Kripke/Hilbert/K45.lean
@@ -5,24 +5,24 @@ namespace LO.Modal
 open Kripke
 open Geachean
 
-abbrev Kripke.TransitiveEuclideanFrameClass : FrameClass := { F | Transitive F ∧ Euclidean F }
+protected abbrev Kripke.FrameClass.trans_eucl : FrameClass := { F | Transitive F ∧ Euclidean F }
 
 namespace Hilbert.K45
 
-instance Kripke.sound : Sound (Hilbert.K45) (Kripke.TransitiveEuclideanFrameClass) := by
+instance Kripke.sound : Sound (Hilbert.K45) FrameClass.trans_eucl := by
   convert Hilbert.Geach.Kripke.sound (G := {⟨0, 2, 1, 0⟩, ⟨1, 1, 0, 1⟩});
   . exact eq_Geach;
-  . unfold TransitiveEuclideanFrameClass MultiGeacheanConfluentFrameClass MultiGeachean;
+  . unfold FrameClass.trans_eucl FrameClass.multiGeachean MultiGeachean;
     simp [Geachean.euclidean_def, Geachean.transitive_def];
 
 instance Kripke.consistent : Entailment.Consistent (Hilbert.K45) := by
-  convert Hilbert.Geach.Kripke.Consistent (G := {⟨0, 2, 1, 0⟩, ⟨1, 1, 0, 1⟩});
+  convert Hilbert.Geach.Kripke.consistent (G := {⟨0, 2, 1, 0⟩, ⟨1, 1, 0, 1⟩});
   exact eq_Geach;
 
-instance Kripke.canonical : Canonical (Hilbert.K45) (Kripke.TransitiveEuclideanFrameClass) :=
+instance Kripke.canonical : Canonical (Hilbert.K45) FrameClass.trans_eucl :=
   ⟨⟨Canonical.transitive, Canonical.euclidean⟩⟩
 
-instance Kripke.complete : Complete (Hilbert.K45) (Kripke.TransitiveEuclideanFrameClass) := inferInstance
+instance Kripke.complete : Complete (Hilbert.K45) FrameClass.trans_eucl := inferInstance
 
 end Hilbert.K45
 
