Foundation/Modal/Kripke/Hilbert/K4Point2.lean
@@ -7,30 +7,36 @@ open Kripke
 open Geachean
 
 
-abbrev Kripke.TransitiveWeakConfluentFrameClass : FrameClass := { F | Transitive F ∧ WeakConfluent F }
+abbrev Kripke.FrameClass.trans_weakConfluent : FrameClass := { F | Transitive F ∧ WeakConfluent F }
 
-instance Kripke.TransitiveWeakConfluentFrameClass.DefinedByK4Point2Axioms
-  : FrameClass.DefinedBy Kripke.TransitiveWeakConfluentFrameClass Hilbert.K4Point2.axioms := by
+namespace Kripke.FrameClass.trans_weakConnected
+
+protected instance definability_Hilbert
+  : FrameClass.DefinedBy Kripke.FrameClass.trans_weakConfluent Hilbert.K4Point2.axioms := by
   rw [
-    (show TransitiveWeakConfluentFrameClass = TransitiveFrameClass ∩ WeakConfluentFrameClass by aesop),
+    (show Kripke.FrameClass.trans_weakConfluent = FrameClass.trans ∩ FrameClass.weakConfluent by rfl),
     (show Hilbert.K4Point2.axioms = Hilbert.K4.axioms ∪ {Axioms.WeakPoint2 (.atom 0) (.atom 1)} by aesop)
   ];
-  exact FrameClass.definedBy_inter Kripke.TransitiveFrameClass (Hilbert.K4.axioms) WeakConfluentFrameClass {Axioms.WeakPoint2 (.atom 0) (.atom 1)};
+  exact FrameClass.definedBy_inter FrameClass.trans (Hilbert.K4.axioms) FrameClass.weakConfluent {Axioms.WeakPoint2 (.atom 0) (.atom 1)};
 
-instance : Kripke.TransitiveWeakConfluentFrameClass.IsNonempty := by
-  use ⟨Unit, λ _ _ => True⟩;
-  simp [Reflexive, Transitive, WeakConfluent ];
+@[simp]
+protected lemma nonempty : Kripke.FrameClass.trans_weakConfluent.Nonempty := by
+  use whitepoint.toFrame;
+  simp [Transitive, WeakConfluent];
 
-namespace Hilbert.K4Point2
+end Kripke.FrameClass.trans_weakConnected
 
-instance Kripke.sound : Sound (Hilbert.K4Point2) (TransitiveWeakConfluentFrameClass) := inferInstance
 
-instance Kripke.consistent : Entailment.Consistent (Hilbert.K4Point2) := Hilbert.consistent_of_FrameClass TransitiveWeakConfluentFrameClass
+namespace Hilbert.K4Point2.Kripke
 
-instance Kripke.canonical : Canonical (Hilbert.K4Point2) (TransitiveWeakConfluentFrameClass) := ⟨Canonical.transitive, Canonical.weakConfluent⟩
+instance sound : Sound (Hilbert.K4Point2) Kripke.FrameClass.trans_weakConfluent := inferInstance
 
-instance Kripke.complete : Complete (Hilbert.K4Point2) (TransitiveWeakConfluentFrameClass) := inferInstance
+instance consistent : Entailment.Consistent (Hilbert.K4Point2) := Hilbert.consistent_of_FrameClass Kripke.FrameClass.trans_weakConfluent
 
-end Hilbert.K4Point2
+instance canonical : Canonical (Hilbert.K4Point2) Kripke.FrameClass.trans_weakConfluent := ⟨Canonical.transitive, Canonical.weakConfluent⟩
+
+instance complete : Complete (Hilbert.K4Point2) Kripke.FrameClass.trans_weakConfluent := inferInstance
+
+end Hilbert.K4Point2.Kripke
 
 end LO.Modal
