Foundation/Modal/Kripke/Hilbert/KD.lean
@@ -5,23 +5,23 @@ namespace LO.Modal
 open Kripke
 open Geachean
 
-abbrev Kripke.SerialFrameClass : FrameClass := { F | Serial F }
+abbrev Kripke.FrameClass.serial : FrameClass := { F | Serial F }
 
 namespace Hilbert.KD
 
-instance Kripke.sound : Sound (Hilbert.KD) (Kripke.SerialFrameClass) := by
+instance Kripke.sound : Sound (Hilbert.KD) Kripke.FrameClass.serial := by
   convert Hilbert.Geach.Kripke.sound (G := {⟨0, 0, 1, 1⟩});
   . exact eq_Geach;
-  . unfold SerialFrameClass MultiGeacheanConfluentFrameClass MultiGeachean;
+  . unfold Kripke.FrameClass.serial FrameClass.multiGeachean MultiGeachean;
     simp [Geachean.serial_def];
 
 instance Kripke.consistent : Entailment.Consistent (Hilbert.KD) := by
-  convert Hilbert.Geach.Kripke.Consistent (G := {⟨0, 0, 1, 1⟩});
+  convert Hilbert.Geach.Kripke.consistent (G := {⟨0, 0, 1, 1⟩});
   exact eq_Geach;
 
-instance Kripke.canonical : Canonical (Hilbert.KD) (SerialFrameClass) := ⟨Canonical.serial⟩
+instance Kripke.canonical : Canonical (Hilbert.KD) Kripke.FrameClass.serial := ⟨Canonical.serial⟩
 
-instance Kripke.complete : Complete (Hilbert.KD) (SerialFrameClass) := inferInstance
+instance Kripke.complete : Complete (Hilbert.KD) Kripke.FrameClass.serial := inferInstance
 
 end Hilbert.KD
 
