Foundation/Modal/Kripke/Hilbert/KD45.lean
@@ -5,23 +5,23 @@ namespace LO.Modal
 open Kripke
 open Geachean
 
-abbrev Kripke.SerialTransitiveEuclideanFrameClass : FrameClass := { F | Serial F ∧ Transitive F ∧ Euclidean F }
+abbrev Kripke.FrameClass.serial_trans_eucl : FrameClass := { F | Serial F ∧ Transitive F ∧ Euclidean F }
 
 namespace Hilbert.KD45
 
-instance Kripke.sound : Sound (Hilbert.KD45) (Kripke.SerialTransitiveEuclideanFrameClass) := by
+instance Kripke.sound : Sound (Hilbert.KD45) Kripke.FrameClass.serial_trans_eucl := by
   convert Hilbert.Geach.Kripke.sound (G := {⟨0, 0, 1, 1⟩, ⟨0, 2, 1, 0⟩, ⟨1, 1, 0, 1⟩});
   . exact eq_Geach;
-  . unfold SerialTransitiveEuclideanFrameClass MultiGeacheanConfluentFrameClass MultiGeachean;
+  . unfold Kripke.FrameClass.serial_trans_eucl FrameClass.multiGeachean MultiGeachean;
     simp [Geachean.serial_def, Geachean.euclidean_def, Geachean.transitive_def];
 
 instance Kripke.consistent : Entailment.Consistent (Hilbert.KD45) := by
-  convert Hilbert.Geach.Kripke.Consistent (G := {⟨0, 0, 1, 1⟩, ⟨0, 2, 1, 0⟩, ⟨1, 1, 0, 1⟩});
+  convert Hilbert.Geach.Kripke.consistent (G := {⟨0, 0, 1, 1⟩, ⟨0, 2, 1, 0⟩, ⟨1, 1, 0, 1⟩});
   exact eq_Geach;
 
-instance Kripke.canonical : Canonical (Hilbert.KD45) (SerialTransitiveEuclideanFrameClass) := ⟨⟨Canonical.serial, Canonical.transitive, Canonical.euclidean⟩⟩
+instance Kripke.canonical : Canonical (Hilbert.KD45) Kripke.FrameClass.serial_trans_eucl := ⟨⟨Canonical.serial, Canonical.transitive, Canonical.euclidean⟩⟩
 
-instance Kripke.complete : Complete (Hilbert.KD45) (SerialTransitiveEuclideanFrameClass) := inferInstance
+instance Kripke.complete : Complete (Hilbert.KD45) Kripke.FrameClass.serial_trans_eucl := inferInstance
 
 end Hilbert.KD45
 
