Foundation/Modal/Kripke/Hilbert/KDB.lean
@@ -5,23 +5,23 @@ namespace LO.Modal
 open Kripke
 open Geachean
 
-abbrev Kripke.SerialSymmetricFrameClass : FrameClass := { F | Serial F ∧ Symmetric F }
+abbrev Kripke.FrameClass.serial_symm : FrameClass := { F | Serial F ∧ Symmetric F }
 
 namespace Hilbert.KDB
 
-instance Kripke.sound : Sound (Hilbert.KDB) (Kripke.SerialSymmetricFrameClass) := by
+instance Kripke.sound : Sound (Hilbert.KDB) Kripke.FrameClass.serial_symm := by
   convert Hilbert.Geach.Kripke.sound (G := {⟨0, 0, 1, 1⟩, ⟨0, 1, 0, 1⟩});
   . exact eq_Geach;
-  . unfold SerialSymmetricFrameClass MultiGeacheanConfluentFrameClass MultiGeachean;
+  . unfold Kripke.FrameClass.serial_symm FrameClass.multiGeachean MultiGeachean;
     simp [Geachean.serial_def, Geachean.symmetric_def];
 
 instance Kripke.consistent : Entailment.Consistent (Hilbert.KDB) := by
-  convert Hilbert.Geach.Kripke.Consistent (G := {⟨0, 0, 1, 1⟩, ⟨0, 1, 0, 1⟩});
+  convert Hilbert.Geach.Kripke.consistent (G := {⟨0, 0, 1, 1⟩, ⟨0, 1, 0, 1⟩});
   exact eq_Geach;
 
-instance Kripke.canonical : Canonical (Hilbert.KDB) (SerialSymmetricFrameClass) := ⟨⟨Canonical.serial, Canonical.symmetric⟩⟩
+instance Kripke.canonical : Canonical (Hilbert.KDB) Kripke.FrameClass.serial_symm := ⟨⟨Canonical.serial, Canonical.symmetric⟩⟩
 
-instance Kripke.complete : Complete (Hilbert.KDB) (SerialSymmetricFrameClass) := inferInstance
+instance Kripke.complete : Complete (Hilbert.KDB) Kripke.FrameClass.serial_symm := inferInstance
 
 end Hilbert.KDB
 
