Foundation/Modal/Logic/Sublogic/KH.lean
@@ -9,11 +9,11 @@ open Kripke
 theorem K_ssubset_KH : Logic.K ⊂ Logic.KH := by
   constructor;
   . exact Hilbert.weakerThan_of_dominate_axioms (by simp) |>.subset;
-  . suffices ∃ φ, Hilbert.KH ⊢! φ ∧ ¬AllFrameClass ⊧ φ by simpa [K.eq_AllKripkeFrameClass_Logic];
+  . suffices ∃ φ, Hilbert.KH ⊢! φ ∧ ¬FrameClass.all ⊧ φ by simpa [K.eq_AllKripkeFrameClass_Logic];
     use (Axioms.H (.atom 0));
     constructor;
     . exact axiomH!;
-    . apply Formula.Kripke.ValidOnFrameClass.not_of_exists_model_world;
+    . apply Kripke.not_validOnFrameClass_of_exists_model_world;
       use ⟨⟨Fin 1, λ x y => True⟩, λ w _ => False⟩, 0;
       simp [Satisfies, Semantics.Realize];
       constructor <;> tauto;
